\documentclass{article}
\usepackage[utf8]{inputenc}
\usepackage{amsmath,amssymb}
\usepackage{amsfonts,latexsym,cancel}
\title{PIA}
\author{Team 5}
\date{June, 2nd 2021}

\begin{document}

\maketitle
\begin{list}{}{}
       \item MEMBERS:
       \item ABNER ZAIR VELAZQUEZ DOMINGUEZ 1960233 ITS
       \item ALFREDO PALACIOS TREJO 2077513 IMTC
       \item ALFREDO PALACIOS TREJO 2077513 IMTC
       \item JOSE CARLOS GUTIERREZ ORTEGA 1963389 IMTC
       \item JULIO ANGEL ARIAS BARTOLO 1954467 IMTC
       \item Group: 051 
       \item Hour: M6 
       \item Math II
\end{list}
\newpage
\section{Equation}

\bigskip \textbf{ Find  $\int_{0}^1 f(x)dx $\ }

\bigskip SOLUTION:

\bigskip As team, we decided to use u substitution to get an answer, so we said that $\ f(u) + f({1-\frac{1}{u})}$ = $\arctan{u} $\ 

\bigskip $\ f(u)+f(1-\frac{1}{u}) =  \arctan{u} $\ 

\bigskip So, we use u= 1 - $\frac{1}{x}$ = $\frac{x-1}{x} $\

\bigskip Then, we substitute the values and we get $\ f(\frac{-1}{x-1})+f(x)=\arctan(\frac{-1}{x-1}) $\ 

\bigskip At this part of the moment, we analyze what we can do and we did a u-sub, that $u= \frac{-1}{x-1} $\

\bigskip So, the function: $\ 1-\frac{1}{u}=1-\frac{\frac{1}{-1}}{x-1} =1+(x-1)=x $\

\bigskip \textbf{Going back to the function, we substitute $u= \frac{-1}{x-1} $\ to get:}

\bigskip $\ f(\frac{-1}{x-1})+f(x)=\arctan\frac{-1}{x-1}$

\bigskip \textbf{Results}

\bigskip $\ f(x)+f(1-\frac{1}{x})=\arctan{x} $\

\bigskip $\ -f(1-\frac{1}{x})-f(\frac{-1}{x-1})=-\arctan{1-\frac{1}{x}}$

\bigskip $\ f(\frac{-1}{x-1})+f(x)=\arctan({\frac{-1}{x-1})}$

\newpage

\bigskip \textbf {With the three equations we got, we create an only function to get the definite integral}

\bigskip $\ f(x)+f(1-(\frac{1}{x})-f(1-(\frac{1}{x})-f(\frac{-1}{x-1})+f(\frac{-1}{x-1})+f(x)=\arctan{x}-\arctan({1-\frac{1}{x})+\arctan{(\frac{-1}{x-1})}}$\

\bigskip $\ 2f(x)=\arctan{x}-\arctan{1-(\frac{1}{x})+\arctan{(\frac{-1}{x-1})}}$

\bigskip $\ f(x)=\frac{1}{2}\arctan{x}-\frac{1}{2}\arctan({1-\frac{1}{x})}+\frac{1}{2}\arctan({\frac{-1}{x-1})} $\

\bigskip Find $\ \int_{0}^{1} f(x)\,dx \, f(x)=\frac{1}{2}\arctan{x}-\arctan{(1-\frac{1}{x})+\arctan{(\frac{-1}{x-1})}} $\

\bigskip $\ \frac{1}{2} \int_{0}^{1} \arctan{x}-\arctan{(1-\frac{1}{x})+\arctan{(\frac{-1}{x-1})}}\,dx \, \ $\

\bigskip  $\ \frac{1}{2} \int_{0}^{1} \arctan{x}+\arctan{(1-\frac{1}{x})-arc\cot{(x-1)}}\,dx \, $

\bigskip $\ \int_{0}^{1} \arctan{x}\,dx \,+\frac{1}{2}\int_{0}^{1} \arctan{(\frac{1}{x}-1)}\,dx \,- \frac{1}{2}\int_{0}^{1} arc\cot{(x-1)}\,dx \, $

\bigskip \textbf{Let's integrate!}

\bigskip $\ \frac{1}{2} \int_{0}^{1} \arctan{(x)} \,dx \, $

\bigskip \textbf{(Using integration by parts)}

\bigskip $\ v= \arctan{(x)} \,\,\,\, v'=\frac{dx}{x^2+1} $\

\bigskip $\ v=dx \,\,\,\,\,\,\,\,\, u=x $\

\bigskip $\ =x\arctan{(x)}-\int_{0}^{1} \frac{x}{x^2+1}\,dx \,$

\bigskip $\ u= x^2+1 \,\,\,\,\,\, du= 2x dx $\ 

\bigskip  $\ =\frac{1}{2}x\arctan{x}-\frac{1}{4}ln(x^2+1) $\

\bigskip
\bigskip \textbf{Now let's integrate the other term} 

\bigskip $\ \frac{1}{2} \int_{0}^{1} \arctan{(\frac{1}{x}-1)} \,dx \, $\

\bigskip $\ v= \arctan{(\frac{1}{x}-1)}  \,\,\,\,\,\,\,\,\,\, v'=\frac{dx}{((\frac{1}{x}-1))^2+1)x^2} $\

\bigskip $\ v=dx \,\,\,\,\,\,\,\,\,\,\,\,\,\,\,u=x $\

\bigskip $\ \frac{1}{2} \arctan{(\frac{1}{x}-1)}x-\frac{1}{2} \int_{0}^{1} \frac{dx}{((\frac{1}{x}-1))^2+1)x} \,dx \, $\

\bigskip $\ \frac{1}{2} \int_{0}^{1} \frac{dx}{((\frac{1}{x}-1))^2+1)x} \,dx \, $\ 


\newpage

\bigskip $\ = \frac{1}{2} \int_{0}^{1} \frac{x}{x^2+(1-x)^2} \,dx \, $\ 

\bigskip \textbf{Write} $\ x $\ {as} $\ \frac{1}{4} \ (2x+2(x-1))+ \frac{1}{2} $\ {and put it in separated therms} 

\bigskip $\ \frac{1}{2} \int_{0}^{1} (\frac{(2x+2(x-1))}{4(x^2+(1-x)^2)} + \frac{1}{2(x^2+(1-x)^2)}) \,dx \,$\ 

\bigskip $\ \frac{1}{8} \int_{0}^{1} \frac{(2x+2(x-1))}{x^2+(1-x)^2}\,dx\, + \frac{1}{2} \int_{0}^{1}\frac{1}{x^2+(1-x)^2} \,dx \,$\ 

\bigskip

\bigskip $\ \frac{1}{8} \int_{0}^{1} \frac{(2x+2(x-1))}{x^2+(1-x)^2}\,dx\,$\ 

\bigskip \textbf{Let's make a variable substitution to integrate} 

\bigskip $\ u=x^2+(1-x)^2 \,\,->\,\, \frac {du}{dx}= 2x+2(x-1) \,\,$\ 

\bigskip $\ du=2x+2(x-1) \,dx\,$\

\bigskip \textbf{Now replace the variables} 

\bigskip $\ \frac{1}{8} \int_ \frac {du}{u} $\

\bigskip $\ = \, \frac{1}{8} \ln (u) $\

\bigskip \textbf{Substitute the original values}

\bigskip $\ = \, \frac{1}{8} \ln (x^2+(1-x)^2)  $


\begin{equation*}
   -\frac{1}{2}\int_{0}^{1} arctan(x-1)dx
\end{equation*}

\bigskip\textbf{We can apply integration by substitution:}
\begin{list}{}{}
       \item $w=x-1$  
       \item $dw=dx$
\end{list}

\begin{equation*}
   -\frac{1}{2}\int_{0}^{1}\textrm{arcot}(w)dx
\end{equation*}

\bigskip\textbf{We can apply integration by parts:} $\int {u\frac{{dv}}{{dx}}} dx = uv - \int {\frac{{du}}{{dx}}} vdx$ 
\begin{list}{}{}
       \item $v=\textrm{arccot}(w)$
       \item $du = dw$
       \item $v'=-\frac{dx}{w^2+1}
$
       \item $u=w$
\end{list}

\begin{equation*}
   =(w)\textrm{arccot}(x-1)+\int_{0}^{1}\frac{w}{w^2+1}dw
\end{equation*}
\begin{list}{}{}
       \item $u=w^2+1$
       \item $du=(2w)dw$
\end{list}

\bigskip\textbf{Then, we integrate and we return $w$ to its original value:}
\begin{equation*}
   =-\frac{1}{2}(w)\textrm{arccot}(x)-\frac{1}{4}ln(w^2+1)
\end{equation*}

\begin{equation*}
   =-\frac{1}{2}(x-1)\textrm{arccot}(x-1)-\frac{1}{4}ln((x-1)^2+1)
\end{equation*}

\bigskip \textbf{RESULT:}

\begin{equation*}
    =\frac{1}{2} x \arctan(x) +\frac{1}{2} \arctan(\frac{1}{x}-1) x -\frac{1}{4} \ln{(x^2 +1)} +\frac{1}{8} \ln{[x^2 +(x-1)^2]}
\end{equation*}

\begin{equation*}
        +\frac{2}{4}\arctan(2x-1) -\frac{1}{2}(x-1) \text{arccot} (x-1) -\frac{1}{4}\ln{[(x-1)^2 +1]} \int_0^1
\end{equation*}

\bigskip\textbf{Compute the limits:}
\begin{equation*}
    =\frac{1}{2} (1) \arctan(1) +\frac{1}{2} \arctan(\frac{1}{1}-1) (1) -\frac{1}{4} \ln{(1^2 +1)} +\frac{1}{8} \ln{[1^2 +(1-1)^2]}
\end{equation*}

\begin{equation*}
        +\frac{2}{4}\arctan[2(1)-1)] -\frac{1}{2}(1-1) \text{arccot} (1-1) -\frac{1}{4}\ln{[(1-1)^2 +1]} 
\end{equation*}

\begin{equation*}
    -\frac{1}{2} (0) \arctan(0) -\frac{1}{2} \arctan(\frac{1}{0}-1) (0) +\frac{1}{4} \ln{(0^2 +1)} -\frac{1}{8} \ln{[0^2 +(0-1)^2]}
\end{equation*}

\begin{equation*}
        -\frac{2}{4}\arctan[2(0)-1] +\frac{1}{2}(0-1) \text{arccot} (0-1) +\frac{1}{4}\ln{[(0-1)^2 +1]}
\end{equation*}

\bigskip\textbf{This is the final result:}
\begin{equation*}
    \frac{3\pi}{8} 
\end{equation*}

\end{document} 
